WIP (doesn't compile)

Procedural.dfy
@@ -1,86 +1,92 @@
 
 // Stuff I would want from a standard library
 
-function method absurd<A>(): A
+function method Absurd<A>(): A
   requires false
 {
-  absurd()
+  Absurd()
 }
 
-function method fst<A,B>(p: (A,B)): A { p.0 }
-function method snd<A,B>(p: (A,B)): B { p.1 }
+function method Fst<A,B>(p: (A,B)): A { p.0 }
+function method Snd<A,B>(p: (A,B)): B { p.1 }
 
 datatype List<A> = Cons(A, List<A>) | Nil
 
-function method length(xs: List): nat {
+function method Length(xs: List): nat {
   match xs
     case Nil          => 0
-    case Cons(_, xs') => 1 + length(xs')
+    case Cons(_, xs') => 1 + Length(xs')
 }
 
-function method mapList<A,B>(f: A -> B, xs: List<A>): List<B>
+lemma {:induction xs} SmallerThanList<A>(x: A, xs: List<A>)
+  requires x in Elements(xs)
+  ensures x < xs
+{
+}
+
+function method MapList<A,B>(f: A -> B, xs: List<A>): List<B>
   requires forall x :: f.reads(x) == {}
-  requires forall x :: f.requires(x)
-  ensures length(xs) == length(mapList(f, xs))
+  requires forall x :: x in Elements(xs) ==> f.requires(x)
+  ensures Length(xs) == Length(MapList(f, xs))
 {
   match xs
     case Nil => Nil
-    case Cons(x, xs') => Cons(f(x), mapList(f, xs'))
+    case Cons(x, xs') => Cons(f(x), MapList(f, xs'))
 }
 
-function method zipWith<A,B,C>(f: (A, B) -> C, xs: List<A>, ys: List<B>): List<C>
+function method ZipWith<A,B,C>(f: (A, B) -> C, xs: List<A>, ys: List<B>): List<C>
   requires forall x, y :: f.reads(x, y) == {}
   requires forall x, y :: f.requires(x, y)
-  requires length(xs) == length(ys)
-  ensures  length(zipWith(f, xs, ys)) == length(xs) == length(ys)
+  requires Length(xs) == Length(ys)
+  ensures  Length(ZipWith(f, xs, ys)) == Length(xs) == Length(ys)
 {
   match (xs, ys)
     case (Nil, Nil) => Nil
-    case (Cons(x, xs'), Cons(y, ys')) => Cons(f(x, y), zipWith(f, xs', ys'))
+    case (Cons(x, xs'), Cons(y, ys')) => Cons(f(x, y), ZipWith(f, xs', ys'))
     // proving that mismatched lists are impossible
-    case (Cons(x, xs'), Nil) => assert (length(Cons(x, xs')) != length<A>(Nil)); absurd()
-    case (Nil, Cons(y, ys')) => assert (length(Cons(y, ys')) != length<B>(Nil)); absurd()
+    case (Cons(x, xs'), Nil) => assert (Length(Cons(x, xs')) != Length<A>(Nil)); Absurd()
+    case (Nil, Cons(y, ys')) => assert (Length(Cons(y, ys')) != Length<B>(Nil)); Absurd()
 }
 
-function method foldr<A, B>(b: B, k: (A, B) -> B, xs: List<A>): B
+function method Foldr<A, B>(b: B, k: (A, B) -> B, xs: List<A>): B
   requires forall x, y :: k.reads(x, y) == {}
   requires forall x, y :: k.requires(x, y)
   decreases xs
 {
   match xs
     case Nil => b
-    case Cons(x, xs') => k(x, foldr(b, k, xs'))
+    case Cons(x, xs') => k(x, Foldr(b, k, xs'))
 }
 
-predicate method all<A>(p: A -> bool, xs: List<A>)
+predicate method All<A>(p: A -> bool, xs: List<A>)
   requires forall x :: p.reads(x) == {}
   requires forall x :: p.requires(x)
 {
-  foldr(true, (x, y) => x && y, mapList(p, xs))
+  Foldr(true, (x, y) => x && y, MapList(p, xs))
 }
 
-predicate method any<A>(p: A -> bool, xs: List<A>)
+predicate method Any<A>(p: A -> bool, xs: List<A>)
   requires forall x :: p.reads(x) == {}
   requires forall x :: p.requires(x)
 {
-  foldr(false, (x, y) => x || y, mapList(p, xs))
+  Foldr(false, (x, y) => x || y, MapList(p, xs))
 }
 
-predicate method and(xs: List<bool>) {
-  all(x => x, xs)
+predicate method And(xs: List<bool>) {
+  All(x => x, xs)
 }
 
-predicate method or(xs: List<bool>) {
-  any(x => x, xs)
+predicate method Or(xs: List<bool>) {
+  Any(x => x, xs)
 }
 
-function method union<A>(xs: List<set<A>>): set<A> {
-  foldr({}, ((x, y) => x + y), xs)
+function method Union<A>(xs: List<set<A>>): set<A> {
+  Foldr({}, ((x, y) => x + y), xs)
 }
 
 datatype Maybe<A> = Just(A) | Nothing
 
-function method mapMaybe<A,B>(x: Maybe<A>, f: A -> B): Maybe<B>
+function method MapMaybe<A,B>(x: Maybe<A>, f: A -> B): Maybe<B>
   requires forall x :: f.reads(x) == {}
   requires forall x :: f.requires(x)
 {
@@ -89,7 +95,7 @@ function method mapMaybe<A,B>(x: Maybe<A>, f: A -> B): Maybe<B>
     case Just(x) => Just(f(x))
 }
 
-function method bindMaybe<A,B>(x: Maybe<A>, f: A -> Maybe<B>): Maybe<B>
+function method BindMaybe<A,B>(x: Maybe<A>, f: A -> Maybe<B>): Maybe<B>
   requires forall x :: f.reads(x) == {}
   requires forall x :: f.requires(x)
 {
@@ -98,8 +104,8 @@ function method bindMaybe<A,B>(x: Maybe<A>, f: A -> Maybe<B>): Maybe<B>
     case Just(x) => f(x)
 }
 
-function method isJust<A>(x: Maybe<A>): bool
-  ensures (exists y :: x == Just(y)) <==> isJust(x)
+function method IsJust<A>(x: Maybe<A>): bool
+  ensures (exists y :: x == Just(y)) <==> IsJust(x)
 {
   match x
     case Just(_) => true
@@ -108,7 +114,7 @@ function method isJust<A>(x: Maybe<A>): bool
 
 datatype Either<A,B> = Left(A) | Right(B)
 
-function method either<A,B,R>(f: A -> R, g: B -> R, e: Either<A,B>): R
+function method Either<A,B,R>(f: A -> R, g: B -> R, e: Either<A,B>): R
   requires forall a :: f.reads(a) == {}
   requires forall b :: g.reads(b) == {}
   requires forall a :: f.requires(a)
@@ -119,20 +125,19 @@ function method either<A,B,R>(f: A -> R, g: B -> R, e: Either<A,B>): R
     case Right(r) => g(r)
 }
 
-function method lefts<A,B>(es: List<Either<A,B>>): List<A> {
+function method Lefts<A,B>(es: List<Either<A,B>>): List<A> {
   match es
     case Nil                 => Nil
-    case Cons(Left(l),  es') => Cons(l, lefts(es'))
-    case Cons(Right(_), es') => lefts(es')
+    case Cons(Left(l),  es') => Cons(l, Lefts(es'))
+    case Cons(Right(_), es') => Lefts(es')
 }
 
-function method rights<A,B>(es: List<Either<A,B>>): List<B> {
+function method Rights<A,B>(es: List<Either<A,B>>): List<B> {
   match es
     case Nil                 => Nil
-    case Cons(Left(_),  es') => rights(es')
-    case Cons(Right(r), es') => Cons(r, rights(es'))
+    case Cons(Left(_),  es') => Rights(es')
+    case Cons(Right(r), es') => Cons(r, Rights(es'))
 }
-
 // SYNTAX
 
 type Id = int
@@ -144,28 +149,7 @@ datatype Expr = Unit | False | True | Literal(int) | Id(Id)
               | IfThenElse(Expr, Expr, Expr)
               | Call(Id, List<Expr>)
 
-function method FV_Gamma_Expr(e: Expr): set<Id>
-  decreases e
-{
-  match e
-    case Unit                   => {}
-    case False                  => {}
-    case True                   => {}
-    case Literal(_)             => {}
-    case Id(id)                 => {id}
-    case Not(e1)                => FV_Gamma_Expr(e1)
-    case Apply(e1, _, e2)       => FV_Gamma_Expr(e1) + FV_Gamma_Expr(e2)
-    case IfThenElse(e1, e2, e3) => FV_Gamma_Expr(e1) + FV_Gamma_Expr(e2) + FV_Gamma_Expr(e3)
-    case Call(_, es)            => FV_Gamma_Expr_List(es) // union(mapList(e => FV_Gamma_Expr(e), es))
-}
 
-function method FV_Gamma_Expr_List(es: List<Expr>): set<Id>
-  decreases es
-{
-  match es
-    case Nil => {}
-    case Cons(e, es') => FV_Gamma_Expr(e) + FV_Gamma_Expr_List(es')
-}
 
 datatype Op = RelOp(RelOp) | BoolOp(BoolOp) | MathOp(MathOp)
 
@@ -194,6 +178,33 @@ datatype Statement = Var(Id, Type)
                    | Read(Maybe<Id>, Type)
                    | Print(FormatString, List<Expr>)
 
+type FormatString = List<Either<Type, string>>
+
+// FREE VARIABLES
+
+function method FV_Gamma_Expr(e: Expr): set<Id>
+  decreases e
+{
+  match e
+    case Unit                   => {}
+    case False                  => {}
+    case True                   => {}
+    case Literal(_)             => {}
+    case Id(id)                 => {id}
+    case Not(e1)                => FV_Gamma_Expr(e1)
+    case Apply(e1, _, e2)       => FV_Gamma_Expr(e1) + FV_Gamma_Expr(e2)
+    case IfThenElse(e1, e2, e3) => FV_Gamma_Expr(e1) + FV_Gamma_Expr(e2) + FV_Gamma_Expr(e3)
+    case Call(_, es)            => Union(MapList(e' requires e' < e => FV_Gamma_Expr(e'), es))
+}
+
+function method FV_Gamma_Expr_List(es: List<Expr>): set<Id>
+  decreases es
+{
+  match es
+    case Nil => {}
+    case Cons(e, es') => FV_Gamma_Expr(e) + FV_Gamma_Expr_List(es')
+}
+
 function method FV_Gamma_Statement(s: Statement): set<Id>
 {
   match s
@@ -218,31 +229,12 @@ function method FV_Gamma_Block(ss: Block): set<Id>
     case Cons(s, ss') => FV_Gamma_Statement(s) + FV_Gamma_Block(ss')
 }
 
-type FormatString = List<Either<Type, string>>
 
 // TYPING
 
 datatype Purity = Pure | Impure
 
 datatype Certainty = Yes | Perhaps
-
-function method boolFromCertainty(c: Certainty): bool {
-  match c
-    case Yes => true
-    case Perhaps => false
-}
-
-function method certaintyFromBool(b: bool): Certainty {
-  if b then Yes else Perhaps
-}
-
-function method CertAnd(c1: Certainty, c2: Certainty): Certainty {
-  certaintyFromBool(boolFromCertainty(c1) && boolFromCertainty(c2))
-}
-
-function method CertOr(c1: Certainty, c2: Certainty): Certainty {
-  certaintyFromBool(boolFromCertainty(c1) || boolFromCertainty(c2))
-}
 
 type Delta = map<Id, (List<Type>, Type, Purity)> // env. of declarations
 
@@ -280,59 +272,18 @@ predicate method TypeExpr(delta: Delta, gamma: Gamma, e: Expr, t: Type) {
 
 predicate method TypeList(delta: Delta, gamma: Gamma, es: List<Expr>, ts: List<Type>)
 {
-  length(es) == length(ts) &&
+  Length(es) == Length(ts) &&
     (match (es, ts)
       case (Nil, Nil) => true
-      case (Cons(x, xs'), Nil) => assert (length(Cons(x, xs')) != length<Expr>(Nil)); absurd()
-      case (Nil, Cons(y, ys')) => assert (length(Cons(y, ys')) != length<Type>(Nil)); absurd()
+      case (Cons(x, xs'), Nil) => assert (Length(Cons(x, xs')) != Length<Expr>(Nil)); Absurd()
+      case (Nil, Cons(y, ys')) => assert (Length(Cons(y, ys')) != Length<Type>(Nil)); Absurd()
       case (Cons(e, es'), Cons(t, ts')) =>
         TypeExpr(delta, gamma, e, t) && TypeList(delta, gamma, es', ts'))
   // and(zipWith((e, t) => TypeExpr(delta, gamma, e, t), es, ts))
 }
 
-// predicate TypeStatement(delta: Delta, gamma: Gamma, rho: Type, s: Statement, gamma': Gamma)
-//   decreases s
-// {
-//   match s
-//     case Var(id, t) =>
-//       id !in gamma &&
-//       gamma' == gamma[id := t]
-//     case Assign(id, e) =>
-//       id in gamma &&
-//       TypeExpr(delta, gamma, e, gamma[id])
-//     case IfThenElse(e, s1, s2) =>
-//       TypeExpr(delta, gamma, e, Bool) &&
-//       TypeBlock(delta, gamma, rho, s1, gamma') &&
-//       TypeBlock(delta, gamma, rho, s1, gamma')
-//     case While(e, s) =>
-//       TypeExpr(delta, gamma, e, Bool) &&
-//       TypeBlock(delta, gamma, rho, s, gamma)
-//     case Call(maybeId, id, arguments) =>
-//       id in delta &&
-//       var (argTypes, retType, purity) := delta[id];
-//         (match maybeId
-//           case Just(v) => v in gamma && gamma[v] == retType
-//           case Nothing => true) &&
-//         TypeList(delta, gamma, arguments, argTypes)
-//     case Return(e) =>
-//       TypeExpr(delta, gamma, e, rho)
-//     case Read(maybeId, t) =>
-//       (match maybeId
-//         case Nothing => true
-//         case Just(v) =>
-//           v in gamma && gamma[v] == t)
-//     case Print(spec, arguments) =>
-//       TypeList(delta, gamma, arguments, lefts(spec))
-// }
-
 function method CheckStatement(delta: Delta, gamma: Gamma, rho: Type, s: Statement): Maybe<Gamma>
   decreases s
-  // soundness
-  // ensures forall gamma' :: CheckStatement(delta, gamma, rho, s) == Just(gamma')
-  //                 ==> TypeStatement(delta, gamma, rho, s, gamma')
-  // completeness (TODO: this isn't true yet -- need to prune domain of gamma')
-  // ensures forall gamma' :: TypeStatement(delta, gamma, rho, s, gamma')
-  //                 ==> CheckStatement(delta, gamma, rho, s) == Just(gamma')
 {
   match s
     case Var(id, t) =>
@@ -345,8 +296,8 @@ function method CheckStatement(delta: Delta, gamma: Gamma, rho: Type, s: Stateme
       else Nothing
     case IfThenElse(e, s1, s2) =>
       if !TypeExpr(delta, gamma, e, Bool) then Nothing else
-      bindMaybe(CheckBlock(delta, gamma, rho, s1), gamma1 =>
-      bindMaybe(CheckBlock(delta, gamma, rho, s2), gamma2 =>
+      BindMaybe(CheckBlock(delta, gamma, rho, s1), gamma1 =>
+      BindMaybe(CheckBlock(delta, gamma, rho, s2), gamma2 =>
       if gamma1 == gamma2 then Just(gamma1) else Nothing))
     case While(e, s) =>
       if !TypeExpr(delta, gamma, e, Bool)
@@ -373,39 +324,8 @@ function method CheckStatement(delta: Delta, gamma: Gamma, rho: Type, s: Stateme
       then Just(gamma)
       else Nothing
     case Print(spec, arguments) =>
-      if TypeList(delta, gamma, arguments, lefts(spec)) then Just(gamma) else Nothing
+      if TypeList(delta, gamma, arguments, Lefts(spec)) then Just(gamma) else Nothing
 }
-
-// inductive lemma CheckStatement_sound(delta: Delta, gamma: Gamma, rho: Type, s: Statement, gamma': Gamma)
-//   requires CheckStatement(delta, gamma, rho, s) == Just(gamma')
-//   ensures  TypeStatement(delta, gamma, rho, s, gamma')
-// {
-//   match s
-//     case Var(id, t) =>
-//     case Assign(id, e) =>
-//     case IfThenElse(e, s1, s2) =>
-//       CheckBlock_sound(delta, gamma, rho, s1, gamma');
-//       CheckBlock_sound(delta, gamma, rho, s2, gamma');
-//     case While(e, s) =>
-//       if gamma == gamma' {
-//         CheckBlock_sound(delta, gamma, rho, s, gamma);
-//       }
-//     case Call(maybeId, id, arguments) =>
-//     case Return(e) =>
-//     case Read(maybeId, t) =>
-//     case Print(spec, arguments) =>
-// }
-
-// predicate TypeBlock(delta: Delta, gamma: Gamma, rho: Type, ss: Block, gamma'': Gamma)
-//   decreases ss
-// {
-//   match ss
-//     case Nil => true
-//     case Cons(s, ss') =>
-//       exists gamma' ::
-//         TypeStatement(delta, gamma, rho, s, gamma') &&
-//         TypeBlock(delta, gamma', rho, ss', gamma'')
-// }
 
 function method CheckBlock(delta: Delta, gamma: Gamma, rho: Type, ss: Block): Maybe<Gamma>
   decreases ss
@@ -413,44 +333,23 @@ function method CheckBlock(delta: Delta, gamma: Gamma, rho: Type, ss: Block): Ma
   match ss
     case Nil => Just(gamma)
     case Cons(s, ss') =>
-      bindMaybe(CheckStatement(delta, gamma, rho, s), gamma' =>
+      BindMaybe(CheckStatement(delta, gamma, rho, s), gamma' =>
       CheckBlock(delta, gamma', rho, ss'))
 }
 
-// inductive lemma CheckBlock_sound(delta: Delta, gamma: Gamma, rho: Type, ss: Block, gamma'': Gamma)
-//   requires CheckBlock(delta, gamma, rho, ss) == Just(gamma'')
-//   ensures  TypeBlock(delta, gamma, rho, ss, gamma'')
-// {
-//   match ss
-//     case Nil =>
-//     case Cons(s, ss') =>
-//       var gamma' :| CheckStatement(delta, gamma, rho, s) == Just(gamma');
-//       CheckStatement_sound(delta, gamma, rho, s, gamma');
-//       CheckBlock_sound(delta, gamma', rho, ss', gamma'');
-//       CheckBlock_reassemble(delta, gamma, rho, s, ss', gamma', gamma'');
-// }
-
-// lemma CheckBlock_reassemble(delta: Delta, gamma: Gamma, rho: Type, s: Statement, ss: Block, gamma': Gamma, gamma'': Gamma)
-//   requires CheckBlock(delta, gamma, rho, Cons(s, ss)) == Just(gamma'')
-//   requires TypeStatement(delta, gamma, rho, s, gamma')
-//   requires TypeBlock(delta, gamma', rho, ss, gamma'')
-//   ensures  TypeBlock(delta, gamma, rho, Cons(s, ss), gamma'')
-// {
-// }
-
-predicate method certainBlock(ss: Block)
+predicate method CertainBlock(ss: Block)
 {
   match ss
     case Nil => false
-    case Cons(s, ss') => certainStatement(s) || certainBlock(ss')
-  // any(x => certainStatement(x), ss)
+    case Cons(s, ss') => CertainStatement(s) || CertainBlock(ss')
+  // any(x => CertainStatement(x), ss)
 }
 
-predicate method certainStatement(s: Statement)
+predicate method CertainStatement(s: Statement)
 {
   match s
     case Return(_)             => true
-    case IfThenElse(_, s1, s2) => certainBlock(s1) && certainBlock(s2)
+    case IfThenElse(_, s1, s2) => CertainBlock(s1) && CertainBlock(s2)
     case Var(_, _)             => false
     case Assign(_, _)          => false
     case While(_, _)           => false
@@ -459,21 +358,21 @@ predicate method certainStatement(s: Statement)
     case Print(_, _)           => false
 }
 
-predicate method pureBlock(delta: Delta, ss: Block)
+predicate method PureBlock(delta: Delta, ss: Block)
 {
   match ss
     case Nil => true
-    case Cons(s, ss') => pureStatement(delta, s) && pureBlock(delta, ss')
-  // all(x => pureStatement(delta, x), ss)
+    case Cons(s, ss') => PureStatement(delta, s) && PureBlock(delta, ss')
+  // all(x => PureStatement(delta, x), ss)
 }
 
-predicate method pureStatement(delta: Delta, s: Statement)
+predicate method PureStatement(delta: Delta, s: Statement)
 {
   match s
     case Print(_, _)           => false
     case Read(_, _)            => false
-    case IfThenElse(_, s1, s2) => pureBlock(delta, s1) && pureBlock(delta, s2)
-    case While(_, s)           => pureBlock(delta, s)
+    case IfThenElse(_, s1, s2) => PureBlock(delta, s1) && PureBlock(delta, s2)
+    case While(_, s)           => PureBlock(delta, s)
     case Var(_, _)             => true
     case Assign(_, _)          => true
     case Return(_)             => true
@@ -483,37 +382,54 @@ predicate method pureStatement(delta: Delta, s: Statement)
       purity == Pure)
 }
 
-function method mapFromList<A, B>(pairs: List<(A, B)>): map<A,B> {
-  foldr(map[],
+function method MapFromList<A, B>(pairs: List<(A, B)>): map<A,B> {
+  Foldr(map[],
         ((ab: (A, B), m: map<A,B>) =>
             var (a, b) := ab;
             m[a := b]),
         pairs)
 }
 
-function method elements<A>(xs: List<A>): set<A>
+function method Elements<A>(xs: List<A>): set<A>
 {
-  foldr({}, ((x, s) => {x} + s), xs)
+  Foldr({}, ((x, s) => {x} + s), xs)
 }
 
-predicate method noDuplicates<A(==)>(xs: List<A>) {
-  |elements(xs)| == length(xs)
+predicate method NoDuplicates<A(==)>(xs: List<A>) {
+  |Elements(xs)| == Length(xs)
 }
 
 predicate method TypeDecl(delta: Delta, declaration: Decl) {
-  either(
+  Either(
     ((func: Function) =>
       var Function(args, retType, ss) := func;
-      pureBlock(delta, ss) &&            //            <--- functions must be pure
-      (retType != Type.Unit ==> certainBlock(ss)) &&
-      noDuplicates(mapList(fst, args)) &&
-      isJust(CheckBlock(delta, mapFromList(args), retType, ss))),
+      PureBlock(delta, ss) &&            //            <--- functions must be pure
+      (retType != Type.Unit ==> CertainBlock(ss)) &&
+      NoDuplicates(MapList(Fst, args)) &&
+      IsJust(CheckBlock(delta, MapFromList(args), retType, ss))),
     ((proc: Procedure) =>
       var Procedure(args, retType, ss) := proc;
-      (retType != Type.Unit ==> certainBlock(ss)) &&
-      noDuplicates(mapList(fst, args)) &&
-      isJust(CheckBlock(delta, mapFromList(args), retType, ss))),
+      (retType != Type.Unit ==> CertainBlock(ss)) &&
+      NoDuplicates(MapList(Fst, args)) &&
+      IsJust(CheckBlock(delta, MapFromList(args), retType, ss))),
     declaration)
 }
 
+// BIG STEP SEMANTICS
 
+type State = map<Id, Expr>
+
+predicate method Value(e: Expr) {
+  match e
+    case Unit                => true
+    case False               => true
+    case True                => true
+    case Literal(_)          => true
+    case Id(_)               => false
+    case Not(_)              => false
+    case IfThenElse(_, _, _) => false
+    case Call(_, _)          => false
+    case Apply(_, _, _)      => false
+}
+
+inductive predicate Eval(delta: Delta, s: State, e: Expr, v: Expr)
